src/drf/SmallStep.v
@@ -18,7 +18,7 @@ Require Import Thread.
 Require Import Configuration.
 Require Import Progress.
 
-Require Import MemRel.
+Require Import MemoryRel.
 
 Set Implicit Arguments.
 
