src/opt/Reorder.v
@@ -65,7 +65,7 @@ Lemma reorder_sim_stmts
 Proof.
   pcofix CIH. ii. subst. pfold. ii. splits; ii.
   { inv TERMINAL_TGT. }
-  { exploit sim_local_future; try apply LOCAL; eauto. i. des.
+  { exploit SimPromises.future; try apply LOCAL; eauto. i. des.
     esplits; eauto.
     - etrans.
       + apply Memory.max_timemap_spec; eauto. viewtac.
